src/spec/TLS13.ConnectionState.ProtectedWireSegmentation.fsti
@@ -2,6 +2,8 @@ module TLS13.ConnectionState.ProtectedWireSegmentation
 
 module B = TLS13.Bytes
 module CS = TLS13.Spec.ConnectionState
+module M = TLS13.Messages
+module PWL = TLS13.ConnectionState.ProtectedWireLemmas
 module Seq = FStar.Seq
 
 noextract
@@ -240,4 +242,153 @@ val lemma_paired_replay_suffix_views_from_full_replays_with_equal_prefixes
             client_suffix
             client_suffix_sent
             client_suffix_received
+            client_final)
+
+val lemma_paired_protected_handshake_contiguous_replay_views_from_full_replays_with_equal_prefixes
+  (server_model:CS.connection_model)
+  (client_model:CS.connection_model)
+  (server_prefix:list CS.conn_event)
+  (client_prefix:list CS.conn_event)
+  (server_material:CS.traffic_key_material)
+  (client_material:CS.traffic_key_material)
+  (sent_msg0:M.handshake_msg)
+  (received_msg0:M.handshake_msg)
+  (sent_msg1:M.handshake_msg)
+  (received_msg1:M.handshake_msg)
+  (server_auth_skip:CS.local_event)
+  (client_auth_skip:CS.local_event)
+  (sent_msg2:M.handshake_msg)
+  (received_msg2:M.handshake_msg)
+  (client_verify_skip:CS.local_event)
+  (sent_msg3:M.handshake_msg)
+  (received_msg3:M.handshake_msg)
+  (verified_server_finished:M.finished)
+  (client_app_write_material:CS.traffic_key_material)
+  (client_app_read_material:CS.traffic_key_material)
+  (server_app_write_material:CS.traffic_key_material)
+  (sent_msg4:M.handshake_msg)
+  (received_msg4:M.handshake_msg)
+  (client_finished_rest:list CS.conn_event)
+  (server_finished_rest:list CS.conn_event)
+  (server_full_sent:B.bytes)
+  (server_full_received:B.bytes)
+  (client_full_sent:B.bytes)
+  (client_full_received:B.bytes)
+  (server_final:CS.connection_model)
+  (client_final:CS.connection_model)
+  : Lemma
+      (requires (
+        let server_suffix =
+          PWL.server_protected_handshake_contiguous_replay_events
+            server_material
+            sent_msg0
+            sent_msg1
+            server_auth_skip
+            sent_msg2
+            sent_msg3
+            server_app_write_material
+            received_msg4
+            server_finished_rest in
+        let client_suffix =
+          PWL.client_protected_handshake_contiguous_replay_events
+            client_material
+            received_msg0
+            received_msg1
+            client_auth_skip
+            received_msg2
+            client_verify_skip
+            received_msg3
+            verified_server_finished
+            client_app_write_material
+            client_app_read_material
+            sent_msg4
+            client_finished_rest in
+        Seq.equal server_full_sent client_full_received /\
+        Seq.equal client_full_sent server_full_received /\
+        same_endpoint_replay_split_prefixes_equal
+          server_model
+          server_prefix
+          server_suffix
+          server_full_sent
+          server_full_received
+          server_final /\
+        same_endpoint_replay_split_prefixes_equal
+          client_model
+          client_prefix
+          client_suffix
+          client_full_sent
+          client_full_received
+          client_final /\
+        paired_replay_split_prefixes_equal
+          server_model
+          client_model
+          server_prefix
+          server_suffix
+          client_prefix
+          client_suffix
+          server_full_sent
+          server_full_received
+          client_full_sent
+          client_full_received
+          server_final
+          client_final /\
+        CS.conn_events_sent_seal_replay
+          server_model
+          (FStar.List.Tot.append server_prefix server_suffix)
+          server_full_sent
+          server_full_received
+          server_final /\
+        CS.conn_events_received_decode_replay
+          server_model
+          (FStar.List.Tot.append server_prefix server_suffix)
+          server_full_sent
+          server_full_received
+          server_final /\
+        CS.conn_events_sent_seal_replay
+          client_model
+          (FStar.List.Tot.append client_prefix client_suffix)
+          client_full_sent
+          client_full_received
+          client_final /\
+        CS.conn_events_received_decode_replay
+          client_model
+          (FStar.List.Tot.append client_prefix client_suffix)
+          client_full_sent
+          client_full_received
+          client_final))
+      (ensures
+        exists server_mid client_mid
+          server_raw_sent server_raw_received
+          client_raw_sent client_raw_received.
+          Seq.equal server_raw_sent client_raw_received /\
+          Seq.equal client_raw_sent server_raw_received /\
+          PWL.paired_protected_handshake_contiguous_replay_views
+            server_mid
+            client_mid
+            server_material
+            client_material
+            sent_msg0
+            received_msg0
+            sent_msg1
+            received_msg1
+            server_auth_skip
+            client_auth_skip
+            sent_msg2
+            received_msg2
+            client_verify_skip
+            sent_msg3
+            received_msg3
+            verified_server_finished
+            client_app_write_material
+            client_app_read_material
+            server_app_write_material
+            sent_msg4
+            received_msg4
+            client_finished_rest
+            server_finished_rest
+            server_raw_sent
+            server_raw_received
+            client_raw_sent
+            client_raw_received
+            server_final
             client_final)
